Temp.

rocq-bluerock-brick/theories/lang/cpp/logic/monad.v
@@ -47,20 +47,23 @@ Section with_cpp.
   Context `{Σ : cpp_logic}.
 
   Import linearity.
-
-
   #[local] Opaque FreeTemps.canon.
 
+  (* The type of the continuation *)
+  #[local] Definition K : Type :=
+    forall free : FreeTemps.t, FreeTemps.IsCanonical free -> mpred.
+
   #[local]
-  Lemma K_entails (K : forall free : FreeTemps.t, FreeTemps.IsCanonical free -> mpred)
+  Lemma K_entails (K : K)
     free1 free2 pf1 pf2 :
     free1 ≡ free2 -> K free1 pf1 |-- K free2 pf2.
   Proof. intros. rewrite FreeTemps.K_ext; eauto. Qed.
 
   (* the monad for expression evaluation *)
   Record M {t : Type} := mk
-    { _wp : (t -> forall free : FreeTemps.t, FreeTemps.IsCanonical free -> mpred) -> mpred
-    ; _ok : forall K1 K2, (Forall x free pf, K1 x free pf -* K2 x free pf) |-- _wp K1 -* _wp K2 }.
+    { _wp : (t -> K) -> mpred
+    ; _frame : forall K1 K2, (Forall x free pf, K1 x free pf -* K2 x free pf) |-- _wp K1 -* _wp K2
+    ; _ne : forall K1 K2 n, (forall x y z, K1 x y z ≡{n}≡ K2 x y z) -> _wp K1 ≡{n}≡ _wp K2 }.
   #[global] Arguments M _ : clear implicits.
   #[local] Coercion _wp : M >-> Funclass.
 
@@ -81,8 +84,8 @@ Section with_cpp.
   Proof.
     repeat red. intros.
     split'.
-    { iApply _ok; iIntros (???). rewrite H; eauto. }
-    { iApply _ok; iIntros (???). rewrite H; eauto. }
+    { iApply _frame; iIntros (???). rewrite H; eauto. }
+    { iApply _frame; iIntros (???). rewrite H; eauto. }
   Qed.
   #[global] Instance M_equiv_sym {T} : Symmetric (≡@{M T}).
   Proof.
@@ -102,7 +105,7 @@ Section with_cpp.
     fun a b =>
       forall K1 K2, (forall x y z, K1 x y z ⊢ K2 x y z) -> a K1 ⊢ b K2.
   #[global] Instance M_subseteq_refl {T} : Reflexive (⊆@{M T}).
-  Proof. repeat intro. iApply _ok; iIntros (???); iApply H. Qed.
+  Proof. repeat intro. iApply _frame; iIntros (???); iApply H. Qed.
   #[global] Instance M_subseteq_trans {T} : Transitive (⊆@{M T}).
   Proof.
     repeat intro. etrans.
@@ -133,13 +136,19 @@ Section with_cpp.
   Next Obligation.
     intros; simpl. iIntros "X"; iApply "X".
   Qed.
+  Next Obligation.
+    simpl; intros. apply H.
+  Qed.
   #[global,program]
   Instance Mlocal_map : FMap Mlocal :=
     fun _ _ f m => {| _wp K := m.(_wp) (fun t => K (f <$> t)) |}.
   Next Obligation.
     intros; simpl.
-    iIntros "X"; iApply _ok.
+    iIntros "X"; iApply _frame.
     iIntros (??); iApply "X".
+  Qed.
+  Next Obligation.
+    simpl; intros. apply _ne; eauto.
   Qed.
   #[global,program]
   Instance Mlocal_bind : MBind Mlocal :=
@@ -152,9 +161,13 @@ Section with_cpp.
                                | ReturnVoid => K ReturnVoid f _
                                end) |}.
   Next Obligation.
-    simpl; intros. iIntros "K"; iApply _ok.
-    iIntros (???). case_match; try iApply _ok; eauto.
+    simpl; intros. iIntros "K"; iApply _frame.
+    iIntros (???). case_match; try iApply _frame; eauto.
     iIntros (???); iApply "K".
+  Qed.
+  Next Obligation.
+    simpl; intros.
+    apply _ne; intros. case_match; eauto. apply _ne; simpl; intros; apply H.
   Qed.
 
   #[global,program]
@@ -163,14 +176,20 @@ Section with_cpp.
   Next Obligation.
     intros; simpl. iIntros "X"; iApply "X".
   Qed.
+  Next Obligation.
+    simpl; intros. apply H.
+  Qed.
 
   #[global,program]
   Instance M_map : FMap M :=
     fun _ _ f m => {| _wp K := m.(_wp) (fun t => K (f t)) |}.
   Next Obligation.
     intros; simpl.
-    iIntros "X"; iApply _ok.
+    iIntros "X"; iApply _frame.
     iIntros (??); iApply "X".
+  Qed.
+  Next Obligation.
+    simpl; intros. apply _ne; eauto.
   Qed.
 
   (* Question: Should we implement [ap]? *)
@@ -180,20 +199,22 @@ Section with_cpp.
     fun _ _ k c =>
       {| _wp K := c (fun v f _ => k v (fun v' f' _ => K v' (FreeTemps.canon $ f' >*> f)%free _)) |}.
   Next Obligation.
-    simpl; intros. iIntros "K"; iApply _ok.
-    iIntros (???). iApply _ok. iIntros (???); iApply "K".
+    simpl; intros. iIntros "K"; iApply _frame.
+    iIntros (???). iApply _frame. iIntros (???); iApply "K".
   Qed.
-  Notation "'letWP*' v := e 'in' k" := (M_bind e (fun v => k)) (at level 0, v binder, k at level 200).
+  Next Obligation.
+    simpl; intros. apply _ne; intros. apply _ne; intros. apply H.
+  Qed.
 
   (**  These operations actually form a monad *)
   Lemma mret_mbind {T U} v (k : T -> M U) : mbind k (mret v) ≡ k v.
   Proof.
     red. rewrite /M_equiv/M_bind/M_ret/=. red. simpl; intros.
     split'.
-    { iApply _ok; iIntros (???) "?"; iStopProof.
+    { iApply _frame; iIntros (???) "?"; iStopProof.
       rewrite H; apply K_entails.
       by rewrite FreeTemps.canon_equiv FreeTemps.seq_id_unitR. }
-    { iApply _ok; iIntros (???) "?"; iStopProof.
+    { iApply _frame; iIntros (???) "?"; iStopProof.
       rewrite H; apply K_entails.
       by rewrite FreeTemps.canon_equiv FreeTemps.seq_id_unitR. }
   Qed.
@@ -202,9 +223,9 @@ Section with_cpp.
   Proof.
     red; rewrite /M_equiv/M_bind/M_ret; red; simpl; intros.
     split'.
-    { iApply _ok; iIntros (???) "?"; iStopProof.
+    { iApply _frame; iIntros (???) "?"; iStopProof.
       rewrite H; apply K_entails. rewrite FreeTemps.canon_equiv FreeTemps.seq_left_id; eauto. }
-    { iApply _ok; iIntros (???) "?"; iStopProof.
+    { iApply _frame; iIntros (???) "?"; iStopProof.
       rewrite H; apply K_entails; rewrite FreeTemps.canon_equiv FreeTemps.seq_left_id; eauto. }
   Qed.
 
@@ -213,7 +234,7 @@ Section with_cpp.
   Proof.
     red; rewrite /M_equiv/M_bind; red; simpl; intros.
     split';
-      iApply _ok; iIntros (???); iApply _ok; iIntros (???); iApply _ok; iIntros (???);
+      iApply _frame; iIntros (???); iApply _frame; iIntros (???); iApply _frame; iIntros (???);
       rewrite H; eauto; iIntros; iStopProof; apply K_entails.
     all: rewrite !FreeTemps.canon_equiv FreeTemps.seq_assoc; eauto.
   Qed.
@@ -236,18 +257,18 @@ Section with_cpp.
     m (fun x f _ => Q x f).
  *)
 
-  Definition Knormal {T U} (k : T -> M U) (Q : U -> forall f, FreeTemps.IsCanonical f -> mpred) : T -> forall f, FreeTemps.IsCanonical f -> mpred :=
+  Definition Knormal {T U} (k : T -> M U) (Q : U -> K) : T -> K :=
     fun t free _ => k t (fun u free' _ => Q u (FreeTemps.canon (free' >*> free)) _).
 
   Lemma WP_Mbind {T U} (m : M T) (k : T -> M U) Q :
-    WP m (Knormal k Q) |-- WP (mbind k m) Q.
+    WP m (Knormal k Q) -|- WP (mbind k m) Q.
   Proof.
     rewrite /M_bind/WP/Knormal/=.
-    iApply _ok; iIntros (???). eauto.
+    iSplit; iApply _frame; iIntros (???); eauto.
   Qed.
 
   Lemma WP_ret {T} (v : T) Q :
-    Q v FreeTemps.id _ |-- WP (mret v) Q.
+    Q v FreeTemps.id _ -|- WP (mret v) Q.
   Proof. by rewrite /WP/M_ret/=. Qed.
 
   (** ** The Effects of the Monad
@@ -266,11 +287,17 @@ Section with_cpp.
   Next Obligation.
     intros; simpl. iIntros "X Y P". iApply "X". iApply "Y". iApply "P".
   Qed.
+  Next Obligation.
+    simpl; intros. f_equiv. apply H.
+  Qed.
   #[program]
   Definition Mconsume (P : mpred) : M unit :=
     {| _wp := fun K => P ** K () FreeTemps.id _ |}.
   Next Obligation.
     intros; simpl. iIntros "X [$ K]". iApply "X". iApply "K".
+  Qed.
+  Next Obligation.
+    simpl; intros. f_equiv. apply H.
   Qed.
 
   Lemma WP_produce P Q :
@@ -290,6 +317,9 @@ Section with_cpp.
     simpl; intros.
     iIntros "K X" (?); iApply "K"; eauto.
   Qed.
+  Next Obligation.
+    simpl; intros. f_equiv; intro; eauto.
+  Qed.
   #[program]
   Definition Mangelic (t : Type) : M t :=
     {| _wp K := ∃ x : t, K x FreeTemps.id _ |}%I.
@@ -297,46 +327,56 @@ Section with_cpp.
     simpl; intros.
     iIntros "K X"; iDestruct "X" as (?) "X"; iExists _; iApply "K"; eauto.
   Qed.
+  Next Obligation.
+    simpl; intros. f_equiv; intro; eauto.
+  Qed.
 
   #[program]
   Definition Mub {t : Type} : M t :=
     {| _wp _ := False%I |}.
   Next Obligation. simpl; intros. iIntros "? []". Qed.
+  Next Obligation. simpl; intros. done. Qed.
   #[program]
   Definition Many {t : Type} : M t :=
     {| _wp _ := True%I |}.
   Next Obligation. simpl; intros; iIntros "? ?". iApply bi.pure_intro; [ trivial | ]. iStopProof. reflexivity. Qed.
+  Next Obligation. simpl; intros. done. Qed.
 
   #[program]
   Definition Merror {t : Type} {ERR : Type} (err : ERR) : M t :=
     {| _wp _ := ERROR err |}.
   Next Obligation. simpl; intros. rewrite ERROR_False. iIntros "? []". Qed.
+  Next Obligation. simpl; intros. done. Qed.
 
   #[program]
   Definition Munsupported {t : Type} {ERR : Type} (err : ERR) : M t :=
     {| _wp _ := ERROR err |}.
   Next Obligation. simpl; intros. rewrite ERROR_False. iIntros "? []". Qed.
+  Next Obligation. simpl; intros. done. Qed.
 
   #[program]
   Definition Mpush_free (f : FreeTemps.t) : Mlocal () :=
     {| _wp K := K (Normal ()) (FreeTemps.canon f) _ |}.
   Next Obligation. simpl; intros. iIntros "K"; iApply "K". Qed.
+  Next Obligation. simpl; intros. done. Qed.
 
   #[program]
   Definition Matomically {t} (m : M t) : M t :=
     {| _wp K := |={top,∅}=> m.(_wp) (fun r free _ => |={∅,top}=> K r free _) |}%I.
   Next Obligation.
     simpl; intros. iIntros "K >X !>"; iRevert "X".
-    iApply _ok. iIntros (???) ">X !>"; iRevert "X"; iApply "K".
+    iApply _frame. iIntros (???) ">X !>"; iRevert "X"; iApply "K".
   Qed.
+  Next Obligation. simpl; intros. f_equiv. apply _ne; intros. f_equiv. eauto. Qed.
 
   #[program]
   Definition Mnon_atomically {t} (m : M t) : M t :=
     {| _wp K := |={top}=> m.(_wp) (fun r free _ => |={top}=> K r free _) |}%I.
   Next Obligation.
     simpl; intros. iIntros "K >X !>"; iRevert "X".
-    iApply _ok. iIntros (???) ">X !>"; iRevert "X"; iApply "K".
+    iApply _frame. iIntros (???) ">X !>"; iRevert "X"; iApply "K".
   Qed.
+  Next Obligation. simpl; intros. f_equiv. apply _ne; intros. f_equiv. eauto. Qed.
 
   #[program]
   Definition Mfupd (E1 E2 : coPset): M unit :=
@@ -344,6 +384,7 @@ Section with_cpp.
   Next Obligation.
     simpl; intros. iIntros "K >X !>"; iRevert "X"; iApply "K".
   Qed.
+  Next Obligation. simpl; intros. f_equiv. eauto. Qed.
 
   #[program]
   Definition Mstable : M unit :=
@@ -351,14 +392,16 @@ Section with_cpp.
   Next Obligation.
     simpl; intros. iIntros "K >X !>"; iRevert "X"; iApply "K".
   Qed.
+  Next Obligation. simpl; intros. f_equiv. eauto. Qed.
 
   #[program]
   Definition Mboth {t} (a b : M t) : M t :=
     {| _wp K := a K //\\ b K |}.
   Next Obligation.
     simpl; intros. iIntros "K X".
-    iSplit; [ iDestruct "X" as "[X _]" | iDestruct "X" as "[_ X]" ]; iRevert "X"; iApply _ok; iIntros (??); iApply "K".
+    iSplit; [ iDestruct "X" as "[X _]" | iDestruct "X" as "[_ X]" ]; iRevert "X"; iApply _frame; iIntros (??); iApply "K".
   Qed.
+  Next Obligation. simpl; intros. f_equiv; apply _ne; eauto. Qed.
 
   Definition Mas {T U} (inj : T -> U) (v : U) : M T :=
     letM* p := Mangelic _ in
@@ -377,24 +420,21 @@ Section with_cpp.
     forall Q Q', (Forall x y z, Q x y z -* Q' x y z) ⊢ a Q -* b Q'.
   Definition FrameWith {T} (P : T -> mpred) (a b : M T) : Prop :=
     forall Q Q', (Forall x y z, P x -* Q x y z -* Q' x y z) ⊢ a Q -* b Q'.
-  Notation proper_Frame m := (Frame m m) (only parsing).
 
   Definition FrameI {T} (a b : M T) : mpred :=
     Forall Q Q', (Forall x y z, Q x y z -* Q' x y z) -* a Q -* b Q'.
   Definition FrameWithI {T} (P : T -> mpred) (a b : M T) : mpred :=
     Forall Q Q', (Forall x y z, P x -* Q x y z -* Q' x y z) -* a Q -* b Q'.
 
-  (*
-  Definition Mimpl {T} (a b : M T) : mpred :=
-    ∀ Q, a Q -* b Q.
+  Instance fmap_proper {T U} : Proper (pointwise_relation _ (=) ==> (≡@{M T}) ==> (≡@{M U})) fmap.
+  Proof.
+    repeat intro; rewrite /fmap/=.
+    apply H0.  intros. rewrite H. apply H1.
+  Qed.
 
-  Lemma WP_impl {T} (a b : M T) Q : Mimpl a b |-- WP a Q -* WP b Q.
-  Proof. rewrite /Mimpl. iIntros "X". iApply "X". Qed.
-  *)
-
-  Lemma Mmap_frame_strong {T U} c (f : T -> U) :
-    FrameI c c
-    |-- Forall Q Q', (Forall x y pf, Q (f x) y pf -* Q' (f x) y pf) -* _wp (f <$> c) Q -* _wp (f <$> c) Q'.
+  Lemma Mmap_frame_strong {T U} c1 c2 (f : T -> U) :
+    FrameI c1 c2
+    |-- Forall Q Q', (Forall x y pf, Q (f x) y pf -* Q' (f x) y pf) -* _wp (f <$> c1) Q -* _wp (f <$> c2) Q'.
   Proof.
     rewrite /FrameI/M_map; iIntros "A" (??) "B".
     iApply "A". iIntros (??); iApply "B".
@@ -405,12 +445,6 @@ Section with_cpp.
   Proof.
     rewrite /FrameI/M_map; iIntros "A" (??) "B".
     iApply "A". iIntros (??); iApply "B".
-  Qed.
-
-  Lemma Mframe_refl {T} (m : M T) : proper_Frame m.
-  Proof.
-    rewrite /Frame. iIntros (??) "X".
-    iApply _ok. eauto.
   Qed.
 
   Lemma Mbind_frame {T U} c1 c2 (k1 k2 : T -> M U) :
@@ -427,7 +461,7 @@ Section with_cpp.
       (CITATION NEEDED)
    *)
   #[program]
-  Definition nd_seq {T U} (wp1 : M T) (wp2 : M U) : M (T * U) :=
+  Definition nd_seq {T U} (wp1 : Mlocal T) (wp2 : Mlocal U) : Mlocal (T * U) :=
     Mboth (letM* v1 := wp1 in
            letM* v2 := wp2 in
            mret (v1,v2))
@@ -435,35 +469,83 @@ Section with_cpp.
            letM* v1 := wp1 in
            mret (v1,v2)).
 
+  Instance affinely_intowand {PROP : bi} (R P Q : PROP) : IntoWand false false R P Q -> IntoWand false false (<affine> R) P Q.
+  Proof.
+    rewrite /IntoWand/=.
+    intros. rewrite H. rewrite bi.affinely_elim. done.
+  Qed.
+
+
   Lemma nd_seq_frame {T U} wp1 wp2 :
-    FrameI wp1 wp1 |-- FrameI wp2 wp2 -* FrameI (@nd_seq T U wp1 wp2) (nd_seq wp1 wp2).
+    <affine> FrameI wp1 wp1 |-- <affine> FrameI wp2 wp2 -* FrameI (@nd_seq T U wp1 wp2) (nd_seq wp1 wp2).
   Proof.
     iIntros "A B" (??) "C D".
     iSplit; [ iDestruct "D" as "[D _]" | iDestruct "D" as "[_ D]" ]; iRevert "D".
-    { rewrite /FrameI. iApply "A". iIntros (???). iApply "B"; iIntros (???). iApply "C". }
-    { iApply "B". iIntros (???). iApply "A"; iIntros (???). iApply "C". }
+    { iApply "A". iIntros (???).
+      case_match; eauto. iApply "B"; iIntros (???); case_match; eauto. }
+    { iApply "B". iIntros (???).
+      case_match; eauto. iApply "A"; iIntros (???); case_match; eauto. }
   Qed.
 
   (* Lifting non-deterministic sequencing to lists.
 
      NOTE: this is like the semantics of argument evaluation in C++.
    *)
-  (*
-  Fixpoint nd_seqs' {T} (f : nat) (qs : list (M T)) {struct f} : M (list T) :=
+  Fixpoint nd_seqs' {T} (f : nat) (qs : list (Mlocal T)) {struct f} : Mlocal (list T) :=
     match qs with
-    | nil => Mret nil
+    | nil => mret nil
     | _ :: _ =>
       match f with
       | 0 => Mub
-      | S f => fun Q =>
-        Forall pre post q, [| qs = pre ++ q :: post |] -*
-               let lpre := length pre in
-               Mbind q (fun t => Mmap (fun ts => firstn lpre ts ++ t :: skipn lpre ts) (nd_seqs' f (pre ++ post))) Q
+      | S f =>
+        letM* '(pre, post, q) := M2local $ Mnd (list (Mlocal T) * list (Mlocal T) * Mlocal T) in
+        letM* '() := M2local $ Mrequire (qs = pre ++ q :: post) in
+        let lpre := length pre in
+        q ≫= (fun t => (fun ts : list T => firstn lpre ts ++ t :: skipn lpre ts) <$> (nd_seqs' f (pre ++ post)))
       end
     end.
-   *)
 
-  Definition nd_seqs {T} (qs : list (M T)) : M (list T). (* := @nd_seqs' T (length qs) qs. *) Admitted.
+  Definition nd_seqs {T} (qs : list (Mlocal T)) : Mlocal (list T) := @nd_seqs' T (length qs) qs.
+
+  Definition on_normal {T} (P : T -> Prop) (rt : ReturnType T) : Prop :=
+    match rt with
+    | Normal v => P v
+    | _ => True
+    end.
+  Definition on_normalI {T} (P : T -> mpred) (rt : ReturnType T) : mpred :=
+    match rt with
+    | Normal v => P v
+    | _ => emp
+    end.
+
+  Lemma nd_seqs'_frame_strong {T} n : forall (ls : list (Mlocal T)),
+      n = length ls ->
+      FrameWith (on_normalI $ fun x => [| length x = length ls |]) (nd_seqs' n ls) (nd_seqs' n ls).
+  Proof.
+    induction n; simpl; intros.
+    { case_match; eauto.
+      subst. simpl.
+      iIntros (??) "X". iApply "X". eauto.
+      iIntros (??) "? []". }
+    { destruct ls. exfalso; simpl in *; congruence.
+      inversion H.
+      iIntros (??) "X Y". iIntros ([[pre post] q]) => /=.
+      iDestruct ("Y" $! (pre,post,q)) as "[% Y]"=> /=; iFrame "%".
+      iRevert "Y"; iApply _frame; iIntros (???).
+      case_match; try iApply "X"; eauto.
+      unfold FrameWith in IHn.
+      specialize (IHn (pre ++ post)).
+      subst.
+      generalize (f_equal length H0) => /=; rewrite !length_app/= => ?.
+      iApply IHn.
+      { rewrite length_app; lia. }
+      rewrite /on_normalI.
+      iIntros ([] ??) "P"; simpl; iApply "X"; eauto.
+      rewrite !length_app/=. iDestruct "P" as "%".
+      iPureIntro.
+      rewrite firstn_length_le; last lia.
+      rewrite length_skipn. lia. }
+  Qed.
 
   (*
   Lemma nd_seqs'_frame_strong {T} n : forall (ls : list (M T)) Q Q',
@@ -534,10 +616,21 @@ Section with_cpp.
         rewrite !length_app /=. lia. }
       iSplitL "a"; eauto. }
   Qed.
+  *)
+  Lemma nd_seqs_frame_strong : forall {T} (ms : list (_ T)),
+      FrameWith (on_normalI (fun x => [| length x = length ms |])) (nd_seqs ms) (nd_seqs ms).
+  Proof.
+    intros; iIntros (??) "K". iApply nd_seqs'_frame_strong; eauto.
+  Qed.
   Lemma nd_seqs_frame : forall {T} (ms : list (_ T)),
-      ([∗list] m ∈ ms, FrameI m m) |-- FrameI (nd_seqs ms) (nd_seqs ms).
-  Proof. intros. by iApply nd_seqs'_frame. Qed.
+      Frame (nd_seqs ms) (nd_seqs ms).
+  Proof.
+    intros; iIntros (??) "K". iApply nd_seqs_frame_strong; eauto.
+    iIntros (???) "P".
+    destruct x; simpl; iApply "K".
+  Qed.
 
+  (*
   (* sanity check on [nd_seq] and [nd_seqs] *)
   Example nd_seq_example : forall {T} (a b : M T),
       Proper (Mrel _) a -> Proper (Mrel _) b ->
@@ -600,29 +693,29 @@ Section with_cpp.
   *)
 
   (** *** sequencing of monadic compuations *)
-  Definition Mseq {T U} (wp1 : M T) (wp2 : M U) : M (T * U) :=
+  Definition Mseq {T U} (wp1 : Mlocal T) (wp2 : Mlocal U) : Mlocal (T * U) :=
     letM* v := wp1 in
     (fun x => (v,x)) <$> wp2.
 
-  Lemma Mseq_frame {T U} wp1 wp2 :
-    FrameI wp1 wp1 |-- FrameI wp2 wp2 -* FrameI (@Mseq T U wp1 wp2) (Mseq wp1 wp2).
+  Lemma Mseq_frame {T U} wp1 wp1' wp2 wp2' :
+    FrameI wp1 wp1' |-- <affine> FrameI wp2 wp2' -* FrameI (@Mseq T U wp1 wp2) (Mseq wp1' wp2').
   Proof.
     iIntros "A B" (??) "C".
-    rewrite /Mseq.
-    iApply (Mbind_frame with "A [B]"); last iAssumption.
-    iIntros (???) "X". iApply (Mmap_frame with "B"). done.
+    rewrite /Mseq/M_bind/=.
+    iApply "A"; iIntros (???); case_match; eauto.
+    iApply "B"; iIntros (???). iApply "C".
   Qed.
 
   (** [seqs es] is sequential evaluation of [es] *)
-  Fixpoint seqs {T} (es : list (M T)) : M (list T) :=
+  Fixpoint seqs {T} (es : list (Mlocal T)) : Mlocal (list T) :=
     match es with
     | nil => mret []
-    | e :: es => (fun '(a,b) => a :: b) <$> (Mseq e (seqs es))
+    | e :: es => (fun '(a,b) => a :: b) <$> Mseq e (seqs es)
     end.
 
-  Lemma seqs_frame_strong {T} : forall (ls : list (M T)) Q Q',
-      ([∗list] m ∈ ls, FrameI m m)%I
-      |-- (Forall x y pf, [| length x = length ls |] -* Q x y pf -* Q' x y pf) -*
+  Lemma seqs_frame_strong {T} : forall (ls : list (Mlocal T)) Q Q',
+      ([∗list] m ∈ ls, <affine> FrameI m m)%I
+      |-- (Forall x y pf, on_normalI (fun x => [| length x = length ls |]) x -* Q x y pf -* Q' x y pf) -*
           (seqs ls Q) -* (seqs ls Q').
   Proof.
     induction ls; simpl; intros.
@@ -630,11 +723,13 @@ Section with_cpp.
     - iIntros "[A AS] K".
       rewrite /M_bind. iApply "A".
       iIntros (???).
-      iApply (IHls with "AS").
-      iIntros (????).
-      iApply "K". simpl. eauto.
+      case_match; try iApply "K"; eauto.
+      { iApply (IHls with "AS"); rewrite /on_normalI/=.
+        iIntros ([]??) "P"; iApply "K"; eauto.
+        iDestruct "P" as "%"; iPureIntro; simpl; eauto. }
   Qed.
 
+  (*
   (** *** interleaving of monadic values
 
       We encode interleaving through concurrency which we represent through
@@ -643,7 +738,7 @@ Section with_cpp.
       NOTE: this is like the semantics of argument evaluation in C
    *)
   #[program]
-  Definition Mpar {T U} (wp1 : M T) (wp2 : M U) : M (T * U) :=
+  Definition Mpar {T U} (wp1 : M T) (wp2 : Mlocal U) : M (T * U) :=
     {| _wp K := Exists Q1 Q2, wp1 Q1 ** wp2 Q2 ** (Forall v1 v2 f1 f2 pf1 pf2, Q1 v1 f1 pf1 -* Q2 v2 f2 pf2 -* K (v1,v2) (FreeTemps.canon (f1 |*| f2)) _) |}.
   Next Obligation.
     simpl; intros.
@@ -694,11 +789,12 @@ Section with_cpp.
       { simpl. eauto. }
       iApply ("KK" $! v1 v2 f1 f2 pf1 pf2 with "[$] [$]").
   Qed.
+  *)
 
   (** *** evaluation by a scheme *)
 
   (** [eval eo e1 e2] evaluates [e1], [e2] according to the evaluation scheme [eo] *)
-  Definition eval2 (eo : evaluation_order.t) {T U} (e1 : M T) (e2 : M U) : M (T * U) :=
+  Definition eval2 (eo : evaluation_order.t) {T U} (e1 : Mlocal T) (e2 : Mlocal U) : Mlocal (T * U) :=
     match eo with
     | evaluation_order.nd => nd_seq e1 e2
     | evaluation_order.l_nd => Mseq e1 e2
@@ -706,50 +802,53 @@ Section with_cpp.
     end.
 
   (** [evals eo es] evaluates [es] according to the evaluation scheme [eo] *)
-  Definition eval (eo : evaluation_order.t) {T} (es : list (M T)) : M (list T) :=
+  Definition eval (eo : evaluation_order.t) {T} (es : list (Mlocal T)) : Mlocal (list T) :=
     match eo with
     | evaluation_order.nd => nd_seqs es
     | evaluation_order.l_nd =>
         match es with
-        | e :: es => letM* v := e in (fun vs => v :: vs) <$> (nd_seqs es)
+        | e :: es => (fun '(a,b) => a :: b) <$> Mseq e (nd_seqs es)
         | [] => mret []
         end
     | evaluation_order.rl => (@rev _) <$> (seqs (rev es))
     end.
 
-  Lemma eval_frame_strong {T} oe : forall (ls : list (M T)) Q Q',
-      ([∗list] m ∈ ls, FrameI m m)%I
-      |-- (Forall x y pf, [| length x = length ls |] -* Q x y pf -* Q' x y pf) -*
+  Lemma eval_frame_strong {T} oe : forall (ls : list (Mlocal T)) Q Q',
+      ([∗list] m ∈ ls, <affine> FrameI m m)%I
+      |-- (Forall x y pf, on_normalI (fun x => [| length x = length ls |]) x -* Q x y pf -* Q' x y pf) -*
           eval oe ls Q -* eval oe ls Q'.
-  Proof. (*
+  Proof.
     destruct oe; intros.
     - rewrite /=/nd_seqs. iIntros "A B".
-      iApply (nd_seqs'_frame_strong with "B A"). done.
-    - simpl.
-      destruct ls; simpl.
+      iApply (nd_seqs'_frame_strong with "B"). done.
+    - destruct ls; simpl.
       { iIntros "_ X"; iApply "X". done. }
       { iIntros "[X Y] K".
-        iApply "X". iIntros (??).
-        iApply (nd_seqs'_frame_strong with "[K] Y"); eauto.
-        iIntros (???).
-        rewrite /Mret.
-        iApply "K". simpl; eauto. }
+        rewrite /Mseq.
+        iApply "X"; iIntros (???).
+        case_match; try iApply "K"; eauto.
+        iApply (nd_seqs'_frame_strong); eauto.
+        iIntros (???) "P".
+        iApply ("K" $! _ _ _).
+        rewrite /on_normalI. destruct x0; simpl; eauto.
+        iDestruct "P" as "%"; iPureIntro; eauto. }
     - simpl.
       iIntros "X K".
-      rewrite /Mmap. iApply (seqs_frame_strong with "[X]").
+      iApply (seqs_frame_strong with "[X]").
       { iStopProof. induction ls; simpl; eauto.
         iIntros "[$ K]".
         iDestruct (IHls with "K") as "$". eauto. }
-      { iIntros (???); iApply "K".
-        rewrite length_rev. eauto. rewrite -(length_rev ls). eauto. }
-  Qed. *) Admitted.
+      { iIntros (???) "P". iApply ("K" $! _ _ _).
+        destruct x; simpl; eauto.
+        rewrite !length_rev. eauto. }
+  Qed.
 
   (** TODO: integrate this *)
   #[global]
   Instance equiv_subseteq_subrelation {T} : @subrelation (M T) (≡) (⊆).
   Proof.
     red. intros. repeat intro.
-    do 2 red in H. rewrite H. iApply _ok. 2: reflexivity.
+    do 2 red in H. rewrite H. iApply _frame. 2: reflexivity.
     iIntros (???). iApply H0.
   Qed.
 
@@ -805,7 +904,7 @@ Section with_cpp.
     m1 ⊆ m2.
   Proof.
     rewrite /WP. repeat intro.
-    rewrite H. iApply _ok. iIntros (???). iApply H0.
+    rewrite H. iApply _frame. iIntros (???). iApply H0.
   Qed.
 
   #[global] Typeclasses Opaque WP M_bind M_ret M_map.
@@ -816,7 +915,7 @@ Section with_cpp.
     intros. red.
     rewrite /M_bind/WP/=.
     f_equiv.
-    iApply _ok. iIntros (???).
+    iApply _frame. iIntros (???).
     iApply K_entails.
     by rewrite FreeTemps.canon_equiv right_id.
   Qed.
@@ -826,7 +925,7 @@ Section with_cpp.
     intros. red.
     rewrite /M_bind/WP/=.
     f_equiv.
-    iApply _ok. iIntros (???).
+    iApply _frame. iIntros (???).
     iApply K_entails.
     by rewrite FreeTemps.canon_equiv right_id.
   Qed.
@@ -836,7 +935,7 @@ Section with_cpp.
   Proof.
     rewrite /WP/Mfupd/=. f_equiv.
     iSplit;
-      by iApply _ok; iIntros (???); iApply K_entails; rewrite FreeTemps.canon_equiv right_id.
+      by iApply _frame; iIntros (???); iApply K_entails; rewrite FreeTemps.canon_equiv right_id.
   Qed.
   Lemma WP_mret {T} (v : T) K :
     WP (mret v) K -|- K v FreeTemps.id _.
@@ -846,14 +945,14 @@ Section with_cpp.
   Proof.
     rewrite /WP/M_bind/M_ret/=.
     iSplit;
-      by iApply _ok; iIntros (???); iApply K_entails; rewrite FreeTemps.canon_equiv right_id.
+      by iApply _frame; iIntros (???); iApply K_entails; rewrite FreeTemps.canon_equiv right_id.
   Qed.
   Lemma WP_Mbind_Mproduce {T} P k K :
     WP (mbind k (Mproduce P)) K -|- P -* WP (T:=T) (k ()) K.
   Proof.
     rewrite /WP/Mproduce/=. f_equiv.
     iSplit;
-      by iApply _ok; iIntros (???); iApply K_entails; rewrite FreeTemps.canon_equiv right_id.
+      by iApply _frame; iIntros (???); iApply K_entails; rewrite FreeTemps.canon_equiv right_id.
   Qed.
 
   (*
@@ -868,7 +967,7 @@ Section with_cpp.
       |-- WP (mbind k1 m) K1 -* WP (mbind k2 m) K2.
   Proof.
     rewrite /WP/M_bind/=.
-    iIntros "k"; iApply _ok; iIntros (???). iApply "k".
+    iIntros "k"; iApply _frame; iIntros (???). iApply "k".
   Qed.
   Hint Opaque Kfree : typeclass_instances.
   Lemma WP_Mbind_Mbind {T U V} m1 (m2 : T -> M U) (m3 : U -> M V) K :
@@ -876,7 +975,7 @@ Section with_cpp.
   Proof.
     rewrite /M_bind/WP/=.
     iSplit;
-      iApply _ok; iIntros (???); iApply _ok; iIntros (???); iApply _ok; iIntros (???);
+      iApply _frame; iIntros (???); iApply _frame; iIntros (???); iApply _frame; iIntros (???);
       iApply K_entails; by rewrite !FreeTemps.canon_equiv assoc.
   Qed.
 
